theories/soundness/call.v
@@ -15,10 +15,8 @@ From shack Require Import eval heap modality interp typing.
 From shack.soundness Require Import expr defs.
 
 Section proofs.
-  (* assume a given set of class definitions *)
-  Context `{PDC: ProgDefContext}.
-  (* assume some SDT constraints and their properties *)
-  Context `{SDTCS: SDTClassSpec}.
+  (* assume a given set of class definitions and their SDT annotations. *)
+  Context `{SDTCVS: SDTClassVarianceSpec}.
 
   (* Helping the inference with this notation that hides pdefs *)
   Local Notation "Δ ⊢ s <: t" := (@subtype _ _ Δ Plain s t) (at level 70, s at next level, no associativity).
@@ -31,407 +29,740 @@ Section proofs.
     wf_cdefs pdefs →
     wf_lty Γ →
     Forall wf_constraint Δ →
+    Forall (bounded_constraint rigid) Δ →
     expr_has_ty Δ Γ rigid kd recv (ClassT exact_ t σ) →
     has_method name t orig mdef →
+    (is_true exact_ ∨ no_this_mdef mdef) →
     mdef.(methodvisibility) = Public →
     dom (methodargs mdef) = dom args →
     (∀ (x : string) (ty : lang_ty) (arg : expr),
        methodargs mdef !! x = Some ty →
        args !! x = Some arg →
-       expr_has_ty Δ Γ rigid kd arg (subst_ty σ ty)) →
+       expr_has_ty Δ Γ rigid kd arg (subst_fty  exact_ t σ ty)) →
+    ∀ t0 t0def Σt0 σ0,
+    pdefs !! t0 = Some t0def →
+    length Σt0 = length t0def.(generics) →
+    inherits_using t0 C σ0 →
     ∀ Σ st st' n,
     length Σ = rigid →
     cmd_eval C st (CallC lhs recv name args) st' n →
+    let Σthis := interp_exact_tag interp_type t0 Σt0 in
+    ⌜interp_list interp_nothing Σt0 σ0 ≡ Σ⌝ -∗
+    □ interp_env_as_mixed Σt0 -∗
     □ interp_env_as_mixed Σ -∗
-    □ Σinterp Σ Δ -∗
-    □ (▷ (∀ (a : tag) (a0 : list constraint) (a1 : subtype_kind)
-            (a2 : nat) (a3 : local_tys) (a4 : cmd)
-            (a5 : local_tys),
-            ⌜wf_lty a3⌝ -∗
-            ⌜bounded_lty a2 a3⌝ -∗
-            ⌜ok_ty a0 (this_type a3)⌝ -∗
-            ⌜Forall wf_constraint a0⌝ -∗
-            ⌜Forall (bounded_constraint a2) a0⌝ -∗
-            ∀ (_ : cmd_has_ty a a0 a1 a2 a3 a4 a5)
-              (x0 : list (interp Θ)) (x1 x2 : local_env * heap)
-              (x3 : nat) (_ : length x0 = a2) (_ : cmd_eval a x1 a4 x2 x3),
-              □ interp_env_as_mixed x0 -∗
-              □ Σinterp x0 a0 -∗
-              heap_models x1.2 ∗ interp_local_tys x0 a3 x1.1 -∗
-              |=▷^x3 heap_models x2.2 ∗ interp_local_tys x0 a5 x2.1)) -∗
-    heap_models st.2 ∗ interp_local_tys Σ Γ st.1 -∗
+    □ Σinterp Σthis Σ Δ -∗
+
+    □ ▷ (∀ C Δ kd rigid Γ cmd Γ',
+         ⌜wf_lty Γ⌝ →
+         ⌜bounded_lty rigid Γ⌝ →
+         ⌜Forall wf_constraint Δ⌝ →
+         ⌜Forall (bounded_constraint rigid) Δ⌝ →
+         ∀ t tdef Σt σ,
+         ⌜pdefs !! t = Some tdef⌝ →
+         ⌜length Σt = length tdef.(generics)⌝ →
+         ⌜inherits_using t C σ⌝ →
+         ⌜cmd_has_ty C Δ kd rigid Γ cmd Γ'⌝ →
+         ∀ Σ st st' n,
+         ⌜length Σ = rigid⌝ →
+         ⌜cmd_eval C st cmd st' n⌝ →
+         ⌜interp_list interp_nothing Σt σ ≡ Σ⌝ -∗
+         □ interp_env_as_mixed Σt -∗
+         □ interp_env_as_mixed Σ -∗
+         □ Σinterp (interp_exact_tag interp_type t Σt) Σ Δ -∗
+         heap_models st.2 ∗
+         interp_local_tys (interp_exact_tag interp_type t Σt) Σ Γ st.1 -∗
+         |=▷^n heap_models st'.2 ∗
+               interp_local_tys (interp_exact_tag interp_type t Σt) Σ Γ' st'.1) -∗
+
+    heap_models st.2 ∗ interp_local_tys Σthis Σ Γ st.1 -∗
     |=▷^n heap_models st'.2 ∗
-          interp_local_tys Σ (<[lhs:=subst_ty σ (methodrettype mdef)]> Γ) st'.1.
+          interp_local_tys Σthis Σ (<[lhs:=subst_fty exact_ t σ (methodrettype mdef)]> Γ) st'.1.
   Proof.
-    move => wfpdefs wflty hΔ hrecv hhasm hpub hdom hi Σ st st' n hrigid hc.
-    iIntros "#hΣ #hΣΔ #IH".
-    elim/cmd_eval_callI : hc.
-    move => {C}{n}.
-    move => Ω h h' l t0 vs vargs orig0 mdef0 run_env run_env' ret n.
-    move => heval_recv hmap hheap hhasm0 hmdom <- heval_body heval_ret /=.
+    move => wfpdefs.
     assert (wfpdefs0 := wfpdefs).
     destruct wfpdefs0.
+    move => wflty hΔ hΔb hrecv hhasm hex hpub hdom hty_args.
+    move => t0 t0def Σt0 σ0 ht0def hlenΣt0 hin_t0_C_σ0.
+    move => Σ st st' n hrigid hc /=.
+    iIntros "%heq #hΣt0 #hΣ #hΣΔ #IH".
+    elim/cmd_eval_callI : hc => {n}.
+    move => Ω h h' l t1 vs vargs orig0 mdef0 run_env run_env' ret n.
+    move => heval_recv hmap hheap hhasm0 hvis hmdom <- heval_body heval_ret.
+    simpl.
     iIntros "[Hh #Hle]".
+    pose (Σthis := interp_exact_tag interp_type t0 Σt0).
+    iAssert (□ interp_as_mixed interp_nothing)%I as "#hnothing".
+    { iModIntro; by iIntros (w) "hw". }
+    iAssert (□ interp_as_mixed Σthis)%I as "#hΣthis".
+    { rewrite /Σthis.
+      iModIntro; iIntros (w) "hw".
+      iLeft; iRight; iRight.
+      iExists t0, Σt0, t0def; iSplit; first done.
+      by iApply (exact_subtype_is_inclusion_aux with "hΣt0 hw").
+    }
     assert (hwfr : wf_ty (ClassT true t σ)).
     { apply expr_has_ty_wf in hrecv => //.
       by eapply wf_ty_exact.
     }
+    assert (hh : ∃ tdef, pdefs !! t = Some tdef ∧ length σ = length tdef.(generics)).
+    { apply wf_tyI in hwfr => //.
+      destruct hwfr as (tdef & ? & ? & ?).
+      by exists tdef; split.
+    }
+    destruct hh as (tdef & htdef & hlenσ).
     (* Get inherits relation between dynamic tag and static tag *)
-    iDestruct (expr_soundness Δ rigid Σ _ recv with "hΣ hΣΔ Hle") as "#Hrecv_" => //.
-    iDestruct (exact_subtype_is_inclusion with "Hrecv_") as "Hrecv"; iClear "Hrecv_".
-    rewrite interp_class_unfold //.
-    iDestruct "Hrecv" as (? t1 def def1 σin Σt fields ifields) "(%Hpure & #hΣt & #hΣtΔ1 & #hf & #hdyn & Hl)".
-    destruct Hpure as ([= <-] & hdef & hdef1 & ? & hin_t1_t & hfields & hidom).
-    iDestruct "Hh" as (sh) "(H● & %Hdom & #Hh)".
-    iDestruct (sem_heap_own_valid_2 with "H● Hl") as "#HΦ".
-    iDestruct ("Hh" with "[//]") as (?) "[H H▷]".
-    iRewrite "H" in "HΦ".
-    rewrite option_equivI prod_equivI /=.
-    iDestruct "HΦ" as "[%Ht HΦ]".
-    fold_leibniz; subst.
-    destruct (has_method_ordered _ _ _ _ _ _ _ _ wf_override wf_parent
-      wf_constraints_bounded wf_methods_bounded hin_t1_t hhasm0 hhasm (*hpub*))
+    iDestruct (expr_soundness Δ rigid Σthis Σ _ recv with "hΣthis hΣ hΣΔ Hle") as "#Hrecv" => //.
+    (* TODO: think of a way to share more of this proof along the two paths
+     * since it's a long one. Still working on it so we'll keep it separated
+     * for now.
+     *)
+    destruct exact_.
+    - (* receiver is an exact type *)
+      rewrite interp_exact_tag_unfold.
+      rewrite (interp_exact_tag_unseal _ t (interp_list Σthis Σ σ)).
+      iDestruct "Hrecv" as (l0 tdef' fields ifields H) "(#hconstr & #hf0 & #H◯)".
+      destruct H as ([= <-] & htdef' & hfields & hidom); simplify_eq.
+      iDestruct "Hh" as (sh) "(H● & %Hdom & #Hh)".
+      iDestruct (sem_heap_own_valid_2 with "H● H◯") as "#HΦ".
+      iDestruct ("Hh" with "[//]") as (?) "[H H▷]".
+      iRewrite "H" in "HΦ".
+      rewrite option_equivI prod_equivI /=.
+      iDestruct "HΦ" as "[%Ht HΦ]".
+      fold_leibniz; subst.
+      destruct (has_method_fun _ _ _ _ _ _ hhasm hhasm0) as [<- <-].
+      assert (h0 := hhasm).
+      apply has_method_from_def in h0 => //.
+      destruct h0 as (odef & omdef & hodef & homdef & hmdef0 & [σin [hin_t_orig ->]]).
+      pose (CT := ClassT false orig (gen_targs (length odef.(generics)))).
+      pose (ΔC := (ThisT, CT) :: odef.(constraints)).
+      assert (hh: wf_mdef_ty orig ΔC (length odef.(generics)) omdef).
+      { apply wf_mdefs in hodef.
+        by apply hodef in homdef.
+      }
+      destruct hh as (Γ' & hwfΓ' & hbody & hret).
+      assert (hwf_lty0 : wf_lty omdef.(methodargs)).
+      { apply wf_methods_wf in hodef.
+        apply hodef in homdef.
+        by apply homdef.
+      }
+      assert (hbounded : bounded_lty (length odef.(generics)) omdef.(methodargs)).
+      { apply wf_methods_bounded in hodef.
+        apply hodef in homdef.
+        by apply homdef.
+      }
+      assert (hwfΔc: Forall wf_constraint ΔC).
+      { apply Forall_cons; split.
+        - split => //=.
+          econstructor => //; first by rewrite length_gen_targs.
+          by apply gen_targs_wf_2.
+        - by apply wf_constraints_wf in hodef.
+      }
+      assert (hbΔc: Forall (bounded_constraint (length odef.(generics))) ΔC).
+      { apply Forall_cons; split.
+        - split => //=.
+          constructor.
+          by apply bounded_gen_targs.
+        - by apply wf_constraints_bounded in hodef.
+      }
+      assert (hΔt : Forall wf_constraint tdef.(constraints)).
+      { by apply wf_constraints_wf in htdef.  }
+      apply cmd_eval_subst in heval_body.
+      rewrite expr_eval_subst in heval_ret.
+      assert (hh: Forall wf_ty σin ∧
+        Forall (bounded (length tdef.(generics))) σin ∧
+        length odef.(generics) = length σin ∧
+        Forall (λ ty : lang_ty, no_this ty) σin).
+      { apply inherits_using_wf in hin_t_orig => //.
+        destruct hin_t_orig as (?&?&?&hh&?); simplify_eq.
+        split; first by apply wf_ty_classI in hh.
+        split; first done.
+        split; last done.
+        apply wf_tyI in hh as (? & ? & ? & ?); by simplify_eq.
+      }
+      destruct hh as (hFσin & hBσin & heq2 & hNTσin).
+      iModIntro; iNext.
+      iAssert (□ interp_env_as_mixed (interp_list Σthis Σ σ))%I as "#hmixed0".
+      { iModIntro; iIntros (k ϕi hk v) "#hv".
+        rewrite /interp_list in hk.
+        apply list_lookup_fmap_inv in hk as [ty [-> hty]].
+        iDestruct (submixed_is_inclusion_aux with "hΣthis hΣ hv") as "hh".
+        - apply wf_ty_classI in hwfr.
+          rewrite Forall_lookup in hwfr.
+          by apply hwfr in hty.
+        - by rewrite interp_mixed_unfold.
+      }
+      iAssert(□ interp_env_as_mixed
+           (interp_list interp_nothing (interp_list Σthis Σ σ) σin))%I as "#hmixed1".
+      { iModIntro; iIntros (k ϕi hk v) "#hv".
+        rewrite /interp_list in hk.
+        apply list_lookup_fmap_inv in hk as [ty [-> hty]].
+        iDestruct (submixed_is_inclusion_aux with "hnothing hmixed0 hv") as "hh".
+        - rewrite Forall_lookup in hFσin.
+          by apply hFσin in hty.
+        - by rewrite interp_mixed_unfold.
+      }
+      assert (hlt : length (interp_list Σthis Σ σ) = length (generics tdef)).
+      { by rewrite /interp_list fmap_length. }
+      iAssert (□ Σinterp (interp_exact_tag interp_type t (interp_list Σthis Σ σ))
+           (interp_list interp_nothing (interp_list Σthis Σ σ) σin) ΔC)%I as "#hΣΔc".
+      { iModIntro.
+        iIntros (k c hc v) "hv".
+        destruct k as [ | k]; simpl in hc.
+        { assert (heq_:
+            interp_list (interp_exact_tag interp_type t (interp_list Σthis Σ σ))
+              (interp_list interp_nothing (interp_list Σthis Σ σ) σin)
+              (gen_targs (length (generics odef))) ≡
+            (interp_list interp_nothing (interp_list Σthis Σ σ) σin)).
+          { apply interp_list_gen_targs.
+            by rewrite /interp_list fmap_length.
+          }
+          case : hc => <- /=.
+          rewrite /ΔC /CT interp_this_unfold interp_tag_unfold.
+          rewrite (interp_tag_equivI _ _ heq_ orig v).
+          iDestruct ((exact_subtype_is_inclusion_aux _ _ _ _ htdef hlt) with "hmixed0 hv") as "hv".
+          by iApply (tag_inherits_using_is_inclusion wf_parent wf_mono
+            wf_fields_wf wf_constraints_wf _ _ _ _ _ _ _ htdef hin_t_orig).
+        }
+        apply inherits_using_ok in hin_t_orig => //.
+        destruct hin_t_orig as (? & ? & hokC); simplify_eq.
+        apply ok_tyI in hokC as(? & ? & ? & hok); simplify_eq.
+        assert (hc' := hc).
+        apply hok in hc'.
+        iDestruct ((subtype_is_inclusion _ hΔt wf_parent wf_mono wf_constraints_wf
+          wf_constraints_no_this wf_constraints_bounded wf_fields_wf
+          _ _ _ _ _ hc' v) with "hnothing hmixed0 hconstr") as "hh".
+        { apply wf_ty_subst; first done.
+          apply wf_constraints_wf in hodef.
+          rewrite /wf_cdef_constraints_wf Forall_lookup in hodef.
+          by apply hodef in hc as [].
+        }
+        assert (hbc: bounded_constraint (length σin) c).
+        { apply wf_constraints_bounded in hodef.
+          rewrite /wf_cdef_constraints_bounded Forall_lookup in hodef.
+          rewrite -heq2.
+          by apply hodef in hc.
+        }
+        destruct hbc as [].
+        rewrite interp_type_subst; last done.
+        rewrite interp_type_subst; last done.
+        apply wf_constraints_no_this in hodef.
+        rewrite /wf_cdef_constraints_no_this Forall_lookup in hodef.
+        apply hodef in hc as [].
+        rewrite (interp_type_no_this _ _ _ (interp_exact_tag interp_type t (interp_list Σthis Σ σ))  interp_nothing); last done.
+        rewrite (interp_type_no_this _ _ _ (interp_exact_tag interp_type t (interp_list Σthis Σ σ))  interp_nothing); last done.
+        by iApply "hh".
+      }
+      assert (hl0 : length (interp_list interp_nothing (interp_list Σthis Σ σ) σin) = length (generics odef)).
+      { by rewrite /interp_list fmap_length heq2. }
+      assert (heqΣ :
+        interp_list interp_nothing (interp_list Σthis Σ σ) σin ≡
+        interp_list interp_nothing (interp_list Σthis Σ σ) σin) by done.
+      iSpecialize ("IH" $! _ _ Plain _ _ _ _ hwf_lty0 hbounded hwfΔc hbΔc).
+      iSpecialize ("IH" $! t tdef (interp_list Σthis Σ σ) σin htdef hlt).
+      iSpecialize ("IH" $! hin_t_orig hbody _ _ _ _ hl0 heval_body heqΣ).
+      iSpecialize ("IH" with "hmixed0 hmixed1 hΣΔc").
+      assert (heq_:
+        interp_list (interp_exact_tag interp_type t (interp_list Σthis Σ σ))
+          (interp_list Σthis Σ σ) σin ≡
+          interp_list interp_nothing (interp_list Σthis Σ σ) σin).
+      { by apply interp_list_no_this. }
+      iDestruct ("IH" with "[Hh Hle H●]") as "Hstep".
+      { iClear "IH"; iSplit.
+        - iExists _; iFrame.
+          iSplit; last done.
+          by rewrite Hdom.
+        - iSplit => /=.
+          + rewrite {2}(interp_exact_tag_unseal _ t (interp_list Σthis Σ σ)).
+            rewrite /interp_exact_tag_def /=.
+            iExists l, tdef, fields, ifields.
+            iSplit; first done.
+            iSplit; first done.
+            by iSplit.
+          + iIntros (v ty hv).
+            assert (ha: ∃ arg, args !! v = Some arg).
+            { apply elem_of_dom.
+              rewrite /subst_mdef /= !dom_fmap_L in hdom.
+              rewrite -hdom.
+              by apply elem_of_dom.
+            }
+            destruct ha as [arg ha].
+            assert (hvarg: ∃ varg, vargs !! v = Some varg).
+            { apply elem_of_dom.
+              apply dom_map_args in hmap.
+              rewrite hmap.
+              apply elem_of_dom.
+              now rewrite ha.
+            }
+            destruct hvarg as [varg hvarg].
+            iExists varg; rewrite hvarg; iSplitR; first done.
+            rewrite (map_args_lookup _ _ _ args vargs hmap v) ha /= in hvarg.
+            assert (h0: methodargs (subst_mdef σin omdef) !! v = Some (subst_ty σin ty)).
+            { by rewrite /subst_mdef /= !lookup_fmap hv. }
+            move: (hty_args v _ _ h0 ha) => haty.
+            iDestruct (expr_soundness with "hΣthis hΣ hΣΔ Hle") as "he" => //.
+            rewrite /subst_fty interp_type_subst; last first.
+            { apply bounded_subst_this; last by (constructor; by apply bounded_gen_targs).
+              eapply bounded_subst => //.
+              - apply wf_methods_bounded in hodef.
+                apply hodef in homdef.
+                by apply homdef in hv.
+              - by rewrite hlenσ.
+            }
+            rewrite hlenσ -hlt.
+            rewrite interp_type_subst_this => //.
+            rewrite interp_type_subst; last first.
+            { apply wf_methods_bounded in hodef.
+              apply hodef in homdef.
+              apply homdef in hv.
+              by rewrite -heq2.
+            }
+            by rewrite (interp_type_equivI _ _ _ heq_).
+      }
+      iRevert "Hstep".
+      iApply updN_mono_I.
+      iIntros "[Hmodels Hle2]"; iFrame.
+      Check interp_local_tys_update.
+      iApply interp_local_tys_update; first by done.
+      rewrite /subst_fty interp_type_subst; last first.
+      { apply bounded_subst_this; last by (constructor; apply bounded_gen_targs).
+        eapply bounded_subst => //.
+        - apply wf_methods_bounded in hodef.
+          apply hodef in homdef.
+          by apply homdef.
+        - by rewrite hlenσ.
+      }
+      rewrite hlenσ -hlt.
+      rewrite interp_type_subst_this => //.
+      rewrite /subst_mdef /= interp_type_subst; last first.
+      { apply wf_methods_bounded in hodef.
+        apply hodef in homdef.
+        rewrite -heq2.
+        by apply homdef.
+      }
+      pose (Σthis_ := interp_exact_tag interp_type t (interp_list Σthis Σ σ)).
+      pose (Σ_ :=
+        interp_list interp_nothing (interp_list Σthis Σ σ) σin).
+      iAssert (□ interp_as_mixed Σthis_)%I as "#HHH0".
+      { rewrite /Σthis_.
+        iModIntro; iIntros (w) "hw".
+        iLeft; iRight; iRight.
+        iExists t, (interp_list Σthis Σ σ), tdef; iSplit; first done.
+        by iApply exact_subtype_is_inclusion_aux.
+      }
+      iDestruct ((expr_soundness ΔC _ Σthis_ Σ_ _ omdef.(methodret) Γ')
+        with "HHH0 hmixed1 hΣΔc Hle2") as "hr" => //.
+      by rewrite (interp_type_equivI _ _ _ heq_).
+    - (* method signature doesn't mention `this` *)
+      case : hex => //= hnothis.
+      rewrite interp_tag_unfold interp_tag_equiv //; last first.
+      { by rewrite /interp_list fmap_length. }
+      iDestruct "Hrecv" as (? t1_ tdef' def1 σin Σt fields ifields) "(%Hpure & #hΣt & #hΣtΔ1 & #hf & #hdyn & Hl)".
+      destruct Hpure as ([= <-] & htdef' & hdef1 & hlen1 & hin_t1_t & hfields & hidom).
+      pose (Σthis1 := interp_exact_tag interp_type t1_ Σt).
+      iAssert (□ ▷ interp_as_mixed Σthis1)%I as "#hmixed1".
+      { rewrite /Σthis1; iModIntro; iNext; iIntros (w) "hw".
+        iLeft; iRight; iRight.
+        iExists t1_, Σt, def1; iSplit; first done.
+        by iApply (exact_subtype_is_inclusion_aux with "hΣt hw").
+      }
+      iAssert (□ ▷ Σinterp Σthis1 Σt (constraints def1))%I as "#hΣtΔ1_".
+      { iModIntro; iNext; iIntros (k c hc w) "hw".
+        apply wf_constraints_no_this in hdef1.
+        assert (hc0 := hc).
+        rewrite /wf_cdef_constraints_no_this Forall_lookup in hdef1.
+        apply hdef1 in hc as [].
+        rewrite (interp_type_no_this _ _ _ Σthis1 interp_nothing); last done.
+        rewrite (interp_type_no_this _ _ _ Σthis1 interp_nothing); last done.
+        by iApply "hΣtΔ1".
+      }
+      iDestruct "Hh" as (sh) "(H● & %Hdom & #Hh)".
+      iDestruct (sem_heap_own_valid_2 with "H● Hl") as "#HΦ".
+      iDestruct ("Hh" with "[//]") as (?) "[H H▷]".
+      iRewrite "H" in "HΦ".
+      rewrite option_equivI prod_equivI /=.
+      iDestruct "HΦ" as "[%Ht HΦ]".
+      fold_leibniz; subst.
+      simplify_eq.
+      destruct (has_method_ordered _ _ _ _ _ _ _ _ wf_override wf_parent
+        wf_constraints_bounded wf_methods_bounded hin_t1_t hhasm0 hhasm (*hpub*))
       as (odef0 & odef & σt1_o0 & σt_o & omdef0 & omdef & hodef0 & hodef & homdef0 & homdef & hin_t1_o0
           & hin_t_o & -> & -> & (*hpub0 &*) hincl0 & _).
-    assert (hwf0: wf_ty (ClassT false orig0 (gen_targs (length odef0.(generics))))).
-    { econstructor => //; last by apply gen_targs_wf_2.
-      by rewrite length_gen_targs.
-    }
-    assert (hh: Forall wf_ty σt_o ∧ length odef.(generics) = length σt_o).
-    { apply inherits_using_wf in hin_t_o => //.
-      destruct hin_t_o as (?&?&?&hh).
-      split; first by apply wf_ty_classI in hh.
-      apply wf_tyI in hh as (? & ? & ? & ?); by simplify_eq.
-    }
-    destruct hh as [hFσt_o heq1].
-    assert (hok0: ok_ty (constraints def1) (ClassT true orig0 σt1_o0)).
-    { apply inherits_using_ok in hin_t1_o0 => //.
-      destruct hin_t1_o0 as (? & ? & ?).
-      by simplify_eq.
-    }
-    assert (hh: wf_mdef_ty orig0 odef0.(constraints) (length odef0.(generics)) (gen_targs (length odef0.(generics))) omdef0).
-    { apply wf_mdefs in hodef0.
-      by apply hodef0 in homdef0.
-    }
-    destruct hh as (Γ' & hwfΓ' & hbody & hret).
-    assert (hwf_lty0 : wf_lty
-    {|
-      type_of_this := (orig0, gen_targs (length odef0.(generics)));
-      ctxt := methodargs omdef0
-    |}).
-    { split => //=.
-      rewrite map_Forall_lookup => k tk hk.
-      apply wf_methods_wf in hodef0.
-      apply hodef0 in homdef0.
-      by apply homdef0 in hk.
-    }
-    assert (hbounded : bounded_lty (length odef0.(generics))
-    {|
-      type_of_this := (orig0, gen_targs (length odef0.(generics)));
-      ctxt := methodargs omdef0
-    |}).
-    { split => /=.
-      - rewrite /this_type /=.
-        constructor.
-        by apply bounded_gen_targs.
-      - rewrite map_Forall_lookup => k tk hk.
-        apply wf_methods_bounded in hodef0.
+      assert (hwf0: wf_ty (ClassT false orig0 (gen_targs (length odef0.(generics))))).
+      { econstructor => //; last by apply gen_targs_wf_2.
+        by rewrite length_gen_targs.
+      }
+      assert (hh: Forall wf_ty σt_o ∧ length odef.(generics) = length σt_o).
+      { apply inherits_using_wf in hin_t_o => //.
+        destruct hin_t_o as (?&?&?&hh&?).
+        split; first by apply wf_ty_classI in hh.
+        apply wf_tyI in hh as (? & ? & ? & ?); by simplify_eq.
+      }
+      destruct hh as [hFσt_o heq1].
+      assert (hok0: ok_ty (constraints def1) (ClassT true orig0 σt1_o0)).
+      { apply inherits_using_ok in hin_t1_o0 => //.
+        destruct hin_t1_o0 as (? & ? & ?).
+        by simplify_eq.
+      }
+      pose (CT := ClassT false orig0 (gen_targs (length odef0.(generics)))).
+      pose (ΔC := (ThisT, CT) :: odef0.(constraints)).
+      assert (hh: wf_mdef_ty orig0 ΔC (length odef0.(generics)) omdef0).
+      { apply wf_mdefs in hodef0.
+        by apply hodef0 in homdef0.
+      }
+      destruct hh as (Γ' & hwfΓ' & hbody & hret).
+      assert (hwf_lty0 : wf_lty omdef0.(methodargs)).
+      { apply wf_methods_wf in hodef0.
         apply hodef0 in homdef0.
-        by apply homdef0 in hk.
-    }
-    assert (hΔ1 : Forall wf_constraint def1.(constraints)).
-    { by apply wf_constraints_wf in hdef1.  }
-    assert (hΔ0 : Forall wf_constraint odef0.(constraints)).
-    { by apply wf_constraints_wf in hodef0. }
-    assert (hΔb0 : Forall (bounded_constraint (length odef0.(generics))) odef0.(constraints)).
-    { by apply wf_constraints_bounded in hodef0. }
-    apply cmd_eval_subst in heval_body.
-    rewrite expr_eval_subst in heval_ret.
-    assert (hh: Forall wf_ty σt1_o0 ∧ length odef0.(generics) = length σt1_o0).
-    { apply inherits_using_wf in hin_t1_o0 => //.
-      destruct hin_t1_o0 as (?&?&?&hh).
-      split; first by apply wf_ty_classI in hh.
-      apply wf_tyI in hh as (? & ? & ? & ?); by simplify_eq.
-    }
-    destruct hh as [hFσt1_o0 heq0].
-    assert (hh: Forall wf_ty σin ∧ length def.(generics) = length σin).
-    { apply inherits_using_wf in hin_t1_t => //.
-      destruct hin_t1_t as (?&?&?&hh).
-      split; first by apply wf_ty_classI in hh.
-      apply wf_tyI in hh as (? & ? & ? & ?); by simplify_eq.
-    }
-    destruct hh as [hFσin heq2].
-    assert (heq3: length def.(generics) = length σ).
-    { apply wf_tyI in hwfr as (? & ? & ? & ?); by simplify_eq. }
-    iModIntro; iNext.
-    iAssert (interp_env_as_mixed (interp_list Σt σt1_o0)) as "hΣt0".
-    { iIntros (k ϕi hk v) "#hv".
-      rewrite /interp_list in hk.
-      apply list_lookup_fmap_inv in hk as [ty [-> hty]].
-      iDestruct (submixed_is_inclusion_aux with "hΣt hv") as "hh".
-      - rewrite Forall_lookup in hFσt1_o0.
-        by apply hFσt1_o0 in hty.
-      - by rewrite interp_mixed_unfold.
-    }
-    iAssert (Σinterp (interp_list Σt σt1_o0) (constraints odef0))%I as "hΣtΔ0".
-    { iIntros (k c hc v) "hv".
-      apply ok_tyI in hok0 as (? & ? & ? & hok0); simplify_eq.
-      assert (hc' := hc).
-      apply hok0 in hc'.
-      iDestruct (subtype_is_inclusion with "hΣt hΣtΔ1") as "hh"; try assumption.
-      { by exact hc'. }
-      { apply wf_ty_subst => //.
-        apply wf_constraints_wf in hodef0.
-        rewrite /wf_cdef_constraints_wf Forall_lookup in hodef0.
-        by apply hodef0 in hc as [].
+        by apply homdef0.
       }
-      assert (hbc: bounded_constraint (length σt1_o0) c).
-      { apply wf_constraints_bounded in hodef0.
-        rewrite /wf_cdef_constraints_bounded Forall_lookup in hodef0.
-        rewrite -heq0.
-        by apply hodef0 in hc.
+      assert (hbounded : bounded_lty (length odef0.(generics)) omdef0.(methodargs)).
+      { apply wf_methods_bounded in hodef0.
+        apply hodef0 in homdef0.
+        by apply homdef0.
       }
-      destruct hbc as [].
-      rewrite interp_type_subst; last done.
-      rewrite interp_type_subst; last done.
-      by iApply "hh".
-    }
-    assert (hconstraints:
-      ∀ (i : nat) (c : lang_ty * lang_ty),
-      subst_constraints σt1_o0 (constraints odef0) !! i = Some c →
-      constraints def1 ⊢ c.1 <D: c.2
-    ).
-    { move => i ? hc.
-      apply list_lookup_fmap_inv in hc as [c [-> hc]].
-      rewrite /subst_constraint /=.
-      apply ok_tyI in hok0 as (? & ? & ? & ?); simplify_eq.
-      by eauto.
-    }
-    destruct hincl0 as [hdom0 [hmargs0 hmret0_]].
-    iDestruct (neg_interp_variance with "hf") as "hf2".
-    assert (hl0 : length (interp_list Σt σt1_o0) = length (generics odef0)).
-    { by rewrite /interp_list fmap_length -heq0. }
-    assert (hwfthis: ok_ty odef0.(constraints)
-                (this_type {| type_of_this := (orig0, gen_targs (length (generics odef0)));
-                              ctxt := methodargs omdef0 |})).
-    { rewrite /this_type /=.
-      econstructor => //.
-      - move => k ty hty.
-        apply lookup_gen_targs in hty as ->.
-        by constructor.
-      - move => k [c0 c1] hc /=.
-        apply wf_constraints_bounded in hodef0.
-        rewrite /wf_cdef_constraints_bounded Forall_lookup in hodef0.
-        rewrite !subst_ty_id.
-        + apply SubConstraint.
-          by apply elem_of_list_lookup_2 in hc.
-        + by apply hodef0 in hc as [].
-        + by apply hodef0 in hc as [].
-    }
-    iSpecialize ("IH" $! _ _ Plain _ _ _ _ hwf_lty0 hbounded hwfthis hΔ0 hΔb0 hbody
-    (interp_list Σt σt1_o0) _ _ _ hl0 heval_body with "hΣt0 hΣtΔ0"); simpl.
-    iDestruct ("IH" with "[Hh Hle H●]") as "Hstep".
-    { iClear "IH"; iSplit.
-      - iExists _; iFrame.
-        iSplit; last done.
-        by rewrite Hdom.
-      - iSplit => /=.
-        + rewrite /interp_this_type interp_this_unseal /interp_this_def /=.
-          iExists l, t1, def1, σt1_o0, Σt, fields, ifields.
-          iSplit; first done.
-          iSplit; first done.
-          iSplit; first done.
-          iSplit; last by iSplit.
-          iPureIntro.
-          rewrite /interp_list.
-          apply equiv_Forall2.
-          rewrite Forall2_lookup => k.
-          rewrite !list_lookup_fmap.
-          destruct (σt1_o0 !! k) as [ty | ] eqn:hty; last first.
-          { rewrite lookup_seq_ge; first done.
-            apply lookup_ge_None_1 in hty.
-            by rewrite heq0.
+      assert (hΔ1 : Forall wf_constraint def1.(constraints)).
+      { by apply wf_constraints_wf in hdef1.  }
+      assert (hΔ0 : Forall wf_constraint ΔC).
+      { apply Forall_cons; by apply wf_constraints_wf in hodef0. }
+      assert (hΔb0 : Forall (bounded_constraint (length odef0.(generics))) ΔC).
+      { apply Forall_cons; split; last by apply wf_constraints_bounded in hodef0.
+        split => //=.
+        constructor; by apply bounded_gen_targs.
+      }
+      apply cmd_eval_subst in heval_body.
+      rewrite expr_eval_subst in heval_ret.
+      assert (hh: Forall wf_ty σt1_o0 ∧
+        length odef0.(generics) = length σt1_o0 ∧
+        Forall no_this σt1_o0).
+      { apply inherits_using_wf in hin_t1_o0 => //.
+        destruct hin_t1_o0 as (?&?&?&hh&?).
+        split; first by apply wf_ty_classI in hh.
+        split; last done.
+        apply wf_tyI in hh as (? & ? & ? & ?); by simplify_eq.
+      }
+      destruct hh as (hFσt1_o0 & heq0 & hNσt1_o0).
+      assert (hh: Forall wf_ty σin ∧
+        Forall (bounded (length def1.(generics))) σin ∧
+        length tdef.(generics) = length σin ∧
+        Forall (λ ty : lang_ty, no_this ty) σin).
+      { apply inherits_using_wf in hin_t1_t => //.
+        destruct hin_t1_t as (?&?&?&hh&?); simplify_eq.
+        split; first by apply wf_ty_classI in hh.
+        split; first done.
+        split; last done.
+        apply wf_tyI in hh as (? & ? & ? & ?); by simplify_eq.
+      }
+      destruct hh as (hFσin & hBσin & heq2 & hNTσin).
+      assert (heq3: length tdef.(generics) = length σ).
+      { apply wf_tyI in hwfr as (? & ? & ? & ?); by simplify_eq. }
+      iModIntro; iNext.
+      iAssert (interp_env_as_mixed (interp_list interp_nothing Σt σt1_o0)) as "hmixed0".
+      { iIntros (k ϕi hk v) "#hv".
+        rewrite /interp_list in hk.
+        apply list_lookup_fmap_inv in hk as [ty [-> hty]].
+        iDestruct (submixed_is_inclusion_aux with "hnothing hΣt hv") as "hh".
+        - rewrite Forall_lookup in hFσt1_o0.
+          by apply hFσt1_o0 in hty.
+        - by rewrite interp_mixed_unfold.
+      }
+      iAssert (Σinterp Σthis1 (interp_list interp_nothing Σt σt1_o0) ΔC)%I as "hΣtΔ0".
+      { iIntros (k c hc v) "hv".
+        destruct k as [ | k]; simpl in hc.
+        { assert (heq_:
+            interp_list Σthis1 (interp_list interp_nothing Σt σt1_o0)
+              (gen_targs (length (generics odef0))) ≡
+            interp_list interp_nothing Σt σt1_o0).
+          { apply interp_list_gen_targs.
+            by rewrite /interp_list fmap_length.
           }
-          rewrite lookup_seq_lt /=; last first.
-          { apply mk_is_Some in hty.
-            apply lookup_lt_is_Some_1 in hty.
-            by rewrite heq0.
-          }
-          constructor => w.
-          by rewrite interp_generic_unfold /interp_generic /= list_lookup_fmap hty /=.
-        + iIntros (v ty hv).
-          assert (ha: ∃ arg, args !! v = Some arg).
-          { apply elem_of_dom.
-            rewrite /subst_mdef /= !dom_fmap_L in hdom0, hmdom.
-            rewrite -hdom /subst_mdef /= dom_fmap -hdom0.
-            by apply elem_of_dom.
-          }
-          destruct ha as [arg ha].
-          assert (hvarg: ∃ varg, vargs !! v = Some varg).
-          { apply elem_of_dom.
-            apply dom_map_args in hmap.
-            rewrite hmap.
-            apply elem_of_dom.
-            now rewrite ha.
-          }
-          destruct hvarg as [varg hvarg].
-          iExists varg; rewrite hvarg; iSplitR; first done.
-          rewrite (map_args_lookup _ _ _ args vargs hmap v) ha /= in hvarg.
-          destruct (methodargs omdef !! v) as [tw | ] eqn:htw; last first.
-          { apply mk_is_Some in hv.
-            apply elem_of_dom in hv.
-            rewrite /subst_mdef /= !dom_fmap_L in hdom0.
-            rewrite hdom0 in hv.
-            apply elem_of_dom in hv.
-            rewrite htw in hv.
-            by elim: hv.
-          }
-          assert (h0: methodargs (subst_mdef σt_o omdef) !! v = Some (subst_ty σt_o tw)).
-          { by rewrite /subst_mdef /= !lookup_fmap htw. }
-          assert (h1 : methodargs (subst_mdef σin (subst_mdef σt_o omdef)) !! v = Some (subst_ty σin (subst_ty σt_o tw))).
-          { by rewrite /subst_mdef /= !lookup_fmap htw. }
-          assert (h2 : methodargs (subst_mdef σt1_o0 omdef0) !! v = Some (subst_ty σt1_o0 ty)).
-          { by rewrite /subst_mdef /= lookup_fmap hv. }
-          assert (hsub: def1.(constraints) ⊢ subst_ty σin (subst_ty σt_o tw) <D: subst_ty σt1_o0 ty).
-          { move: (hmargs0 v _ _ h2 h1) => hsub_.
-            apply subtype_constraint_elim with (Δ' := subst_constraints σt1_o0 odef0.(constraints)) => //.
-            apply subtype_weaken with (Δ := subst_constraints σt1_o0 odef0.(constraints)) => //.
-            by set_solver.
-          }
-          assert (hwf_tw: wf_ty (subst_ty σt_o tw)).
-          { apply wf_ty_subst => //.
-            apply wf_methods_wf in hodef.
-            apply hodef in homdef.
-            by apply homdef in htw.
-          }
-          move: (hi v _ _ h0 ha) => haty.
-          iDestruct (expr_soundness with "hΣ hΣΔ Hle") as "he" => //.
-          assert (hmono: mono (neg_variance <$> def.(generics)) (subst_ty σt_o tw)).
-          { apply mono_subst with (neg_variance <$> odef.(generics)) => //.
-            + apply wf_methods_mono in hodef.
+          case : hc => <- /=.
+          rewrite /ΔC /CT interp_this_unfold interp_tag_unfold.
+          rewrite (interp_tag_equivI _ _ heq_ orig0 v).
+          iDestruct ((exact_subtype_is_inclusion_aux _ _ _ _ hdef1) with "hΣt hv") as "hv".
+          { done. }
+          by iApply (tag_inherits_using_is_inclusion wf_parent wf_mono wf_fields_wf wf_constraints_wf _ _ _ _ _ _ _ hdef1).
+        }
+        apply ok_tyI in hok0 as (? & ? & ? & hok0); simplify_eq.
+        assert (hc' := hc).
+        apply hok0 in hc'.
+        iDestruct ((subtype_is_inclusion _ hΔ1 wf_parent wf_mono wf_constraints_wf
+          wf_constraints_no_this wf_constraints_bounded wf_fields_wf
+          _ _ _ _ _ hc' v) with "hnothing hΣt hΣtΔ1") as "hh".
+        { apply wf_ty_subst; first done.
+          apply wf_constraints_wf in hodef0.
+          rewrite /wf_cdef_constraints_wf Forall_lookup in hodef0.
+          by apply hodef0 in hc as [].
+        }
+        assert (hbc: bounded_constraint (length σt1_o0) c).
+        { apply wf_constraints_bounded in hodef0.
+          rewrite /wf_cdef_constraints_bounded Forall_lookup in hodef0.
+          rewrite -heq0.
+          by apply hodef0 in hc.
+        }
+        destruct hbc as [].
+        rewrite interp_type_subst; last done.
+        rewrite interp_type_subst; last done.
+        apply wf_constraints_no_this in hodef0.
+        rewrite /wf_cdef_constraints_no_this Forall_lookup in hodef0.
+        apply hodef0 in hc as [].
+        rewrite (interp_type_no_this _ _ _ Σthis1 interp_nothing); last done.
+        rewrite (interp_type_no_this _ _ _ Σthis1 interp_nothing); last done.
+        by iApply "hh".
+      }
+      assert (hconstraints:
+        ∀ (i : nat) (c : lang_ty * lang_ty),
+        subst_constraints σt1_o0 (constraints odef0) !! i = Some c →
+        constraints def1 ⊢ c.1 <D: c.2
+      ).
+      { move => i ? hc.
+        apply list_lookup_fmap_inv in hc as [c [-> hc]].
+        rewrite /subst_constraint /=.
+        apply ok_tyI in hok0 as (? & ? & ? & ?); simplify_eq.
+        by eauto.
+      }
+      destruct hincl0 as [hdom0 [hmargs0 hmret0_]].
+      iDestruct (neg_interp_variance with "hf") as "hf2".
+      assert (hl0 : length (interp_list interp_nothing Σt σt1_o0) = length (generics odef0)).
+      { by rewrite /interp_list fmap_length -heq0. }
+      assert (heqΣ: interp_list interp_nothing Σt σt1_o0 ≡
+                    interp_list interp_nothing Σt σt1_o0) by reflexivity.
+      iSpecialize ("IH" $! orig0 _ Plain _ _ _ _ hwf_lty0 hbounded hΔ0 hΔb0).
+      iSpecialize ("IH" $! t1_ def1 Σt _ hdef1 hlen1 hin_t1_o0 hbody).
+      iSpecialize ("IH" $! _ _ _ _ hl0 heval_body heqΣ with "hΣt hmixed0 hΣtΔ0"); simpl.
+      assert (heq_: interp_list interp_nothing Σt σin ≡ interp_list Σthis Σt σin).
+      { by apply interp_list_no_this. }
+      assert (heq_1: interp_list interp_nothing Σt σin ≡ interp_list Σthis1 Σt σin).
+      { by apply interp_list_no_this. }
+      iAssert (□ Σinterp Σthis Σt (constraints def1))%I as "#hΣthisΔ".
+      { iModIntro; iIntros (k c hc w) "hw".
+        apply wf_constraints_no_this in hdef1.
+        rewrite /wf_cdef_constraints_no_this Forall_lookup in hdef1.
+        assert (hc0 := hc).
+        apply hdef1 in hc as [].
+        rewrite (interp_type_no_this _ c.1 _ Σthis interp_nothing); last done.
+        rewrite (interp_type_no_this _ c.2 _ Σthis interp_nothing); last done.
+        iSpecialize ("hΣtΔ1" $! k c hc0 w).
+        by iApply ("hΣtΔ1" with "hw").
+      }
+      iDestruct ("IH" with "[Hh Hle H●]") as "Hstep".
+      { iClear "IH"; iSplit.
+        - iExists _; iFrame.
+          iSplit; last done.
+          by rewrite Hdom.
+        - iSplit => /=.
+          + rewrite (interp_exact_tag_unseal _ t1_ Σt) /interp_exact_tag_def /=.
+            iExists l, def1, fields, ifields.
+            iSplit; first done.
+            iSplit; first done.
+            by iSplit.
+          + iIntros (v ty hv).
+            assert (ha: ∃ arg, args !! v = Some arg).
+            { apply elem_of_dom.
+              rewrite /subst_mdef /= !dom_fmap_L in hdom0, hmdom.
+              rewrite -hdom /subst_mdef /= dom_fmap -hdom0.
+              by apply elem_of_dom.
+            }
+            destruct ha as [arg ha].
+            assert (hvarg: ∃ varg, vargs !! v = Some varg).
+            { apply elem_of_dom.
+              apply dom_map_args in hmap.
+              rewrite hmap.
+              apply elem_of_dom.
+              now rewrite ha.
+            }
+            destruct hvarg as [varg hvarg].
+            iExists varg; rewrite hvarg; iSplitR; first done.
+            rewrite (map_args_lookup _ _ _ args vargs hmap v) ha /= in hvarg.
+            destruct (methodargs omdef !! v) as [tw | ] eqn:htw; last first.
+            { apply mk_is_Some in hv.
+              apply elem_of_dom in hv.
+              rewrite /subst_mdef /= !dom_fmap_L in hdom0.
+              rewrite hdom0 in hv.
+              apply elem_of_dom in hv.
+              rewrite htw in hv.
+              by elim: hv.
+            }
+            assert (h0: methodargs (subst_mdef σt_o omdef) !! v = Some (subst_ty σt_o tw)).
+            { by rewrite /subst_mdef /= !lookup_fmap htw. }
+            assert (h1 : methodargs (subst_mdef σin (subst_mdef σt_o omdef)) !! v = Some (subst_ty σin (subst_ty σt_o tw))).
+            { by rewrite /subst_mdef /= !lookup_fmap htw. }
+            assert (h2 : methodargs (subst_mdef σt1_o0 omdef0) !! v = Some (subst_ty σt1_o0 ty)).
+            { by rewrite /subst_mdef /= lookup_fmap hv. }
+            assert (hsub: def1.(constraints) ⊢ subst_ty σin (subst_ty σt_o tw) <D: subst_ty σt1_o0 ty).
+            { move: (hmargs0 v _ _ h2 h1) => hsub_.
+              apply subtype_constraint_elim with (Δ' := subst_constraints σt1_o0 odef0.(constraints)) => //.
+              apply subtype_weaken with (Δ := subst_constraints σt1_o0 odef0.(constraints)) => //.
+              by set_solver.
+            }
+            assert (hwf_tw: wf_ty (subst_ty σt_o tw)).
+            { apply wf_ty_subst => //.
+              apply wf_methods_wf in hodef.
               apply hodef in homdef.
-              rewrite /wf_mdef_mono hpub in homdef.
               by apply homdef in htw.
-            + rewrite map_length.
-              apply wf_methods_bounded in hodef.
+            }
+            move: (hty_args v _ _ h0 ha) => haty.
+            assert (hno : no_this (subst_ty σt_o tw)).
+            { case: hnothis => hnothis _.
+              by apply hnothis in h0.
+            }
+            rewrite /subst_fty subst_this_no_this_id in haty; last done.
+            iAssert (□ interp_type (subst_ty σ (subst_ty σt_o tw)) Σthis Σ varg)%I as "#he".
+            { iModIntro.
+              by iDestruct (expr_soundness with "hΣthis hΣ hΣΔ Hle") as "he".
+            }
+            assert (hmono: mono (neg_variance <$> tdef.(generics)) (subst_ty σt_o tw)).
+            { apply mono_subst with (neg_variance <$> odef.(generics)) => //.
+              + apply wf_methods_mono in hodef.
+                apply hodef in homdef.
+                rewrite /wf_mdef_mono hpub in homdef.
+                by apply homdef in htw.
+              + rewrite map_length.
+                apply wf_methods_bounded in hodef.
+                apply hodef in homdef.
+                by apply homdef in htw.
+              + by rewrite map_length heq1.
+              + rewrite neg_variance_fmap_idem => i vi ti hvi.
+                apply list_lookup_fmap_inv in hvi.
+                destruct hvi as [wi [-> hwi]].
+                move => hti hc.
+                apply inherits_using_mono with (def := tdef) in hin_t_o => //.
+                elim/mono_classI : hin_t_o => ????; simplify_eq.
+                destruct wi; by eauto.
+              + move => i vi ti hvi.
+                apply list_lookup_fmap_inv in hvi.
+                destruct hvi as [wi [-> hwi]].
+                move => hti hc.
+                apply inherits_using_mono with (def := tdef) in hin_t_o => //.
+                elim/mono_classI : hin_t_o => ????; simplify_eq.
+                destruct wi; by eauto.
+            }
+            assert (hb: bounded (length (generics odef)) tw).
+            { apply wf_methods_bounded in hodef => //.
               apply hodef in homdef.
-              by apply homdef in htw.
-            + by rewrite map_length heq1.
-            + rewrite neg_variance_fmap_idem => i vi ti hvi.
-              apply list_lookup_fmap_inv in hvi.
-              destruct hvi as [wi [-> hwi]].
-              move => hti hc.
-              apply inherits_using_mono with (def := def) in hin_t_o => //.
-              elim/mono_classI : hin_t_o => ????; simplify_eq.
-              destruct wi; by eauto.
-            + move => i vi ti hvi.
-              apply list_lookup_fmap_inv in hvi.
-              destruct hvi as [wi [-> hwi]].
-              move => hti hc.
-              apply inherits_using_mono with (def := def) in hin_t_o => //.
-              elim/mono_classI : hin_t_o => ????; simplify_eq.
-              destruct wi; by eauto.
-          }
-          assert (hb: bounded (length (generics odef)) tw).
-          { apply wf_methods_bounded in hodef => //.
-            apply hodef in homdef.
-            destruct homdef as [hargs _].
-            by apply hargs in htw.
-          }
-          iAssert (interp_type (subst_ty σt_o tw) (interp_list Σt σin) varg)%I as "he2".
-          { iApply (interp_with_mono with "hf2") => //.
-            rewrite interp_type_subst //.
-            apply bounded_subst with (length odef.(generics)) => //.
-            apply inherits_using_wf in hin_t_o => //.
-            destruct hin_t_o as (? & ? & hF & hL); simplify_eq.
-            by rewrite -heq3.
-          }
-          iClear "he hf hf2".
-          rewrite -interp_type_subst; last first.
-          { apply bounded_subst with (length odef.(generics)) => //.
-            apply inherits_using_wf in hin_t_o => //.
-            destruct hin_t_o as (? & ? & hF & hL); simplify_eq.
-            by rewrite -heq2.
-          }
-          iAssert (
-          interp_type (subst_ty σin (subst_ty σt_o tw)) Σt varg-∗
-          interp_type (subst_ty σt1_o0 ty) Σt varg)%I as "hh" .
-          { iApply (subtype_is_inclusion _ hΔ1 wf_parent wf_mono wf_constraints_wf wf_constraints_bounded _ _ _ _ hsub) => //.
-            by apply wf_ty_subst.
-          }
-          rewrite -interp_type_subst; last first.
-          { apply wf_methods_bounded in hodef0.
+              destruct homdef as [hargs _].
+              by apply hargs in htw.
+            }
+            iAssert (interp_type (subst_ty σt_o tw) Σthis (interp_list interp_nothing Σt σin) varg)%I as "he2".
+            { iApply (interp_with_mono with "hf2") => //.
+              rewrite interp_type_subst; first done.
+              apply bounded_subst with (length odef.(generics)) => //.
+              apply inherits_using_wf in hin_t_o => //.
+              destruct hin_t_o as (? & ? & hF & hL); simplify_eq.
+              by rewrite -heq3.
+            }
+            iClear "he hf hf2".
+            rewrite -/Σthis1.
+            rewrite (interp_type_no_this _ _ _ Σthis Σthis1); last done.
+            rewrite (interp_type_equivI _ _ _ heq_1).
+            rewrite -interp_type_subst; last first.
+            { apply bounded_subst with (length odef.(generics)) => //.
+              apply inherits_using_wf in hin_t_o => //.
+              destruct hin_t_o as (? & ? & hF & hL); simplify_eq.
+              by rewrite -heq2.
+            }
+            iAssert (
+              interp_type (subst_ty σin (subst_ty σt_o tw)) Σthis1 Σt varg-∗
+              interp_type (subst_ty σt1_o0 ty) Σthis1 Σt varg)%I as "hh" .
+            { iApply (subtype_is_inclusion _ hΔ1
+              wf_parent wf_mono wf_constraints_wf wf_constraints_no_this
+              wf_constraints_bounded wf_fields_wf _ _ _ _ _ hsub) => //.
+              by apply wf_ty_subst.
+            }
+            iDestruct ("hh" with "he2") as "hh2".
+            iClear "he2 hh".
+            assert (heq__: interp_list interp_nothing Σt σt1_o0 ≡
+                           interp_list Σthis1 Σt σt1_o0).
+            { by apply interp_list_no_this. }
+            rewrite (interp_type_equivI _ _ _ heq__).
+            rewrite interp_type_subst; first done.
+            apply wf_methods_bounded in hodef0.
             apply hodef0 in homdef0.
-            rewrite -heq0.
-            by apply homdef0 in hv.
-          }
-          by iApply "hh".
-    }
-    iRevert "Hstep".
-    iApply updN_mono_I.
-    iIntros "[Hmodels Hle2]"; iFrame.
-    iApply interp_local_tys_update; first by done.
-    assert (hmono: mono def.(generics) (subst_ty σt_o omdef.(methodrettype))).
-    { apply mono_subst with odef.(generics) => //.
-      + apply wf_methods_mono in hodef.
+            apply homdef0 in hv.
+            by rewrite -heq0.
+      }
+      iRevert "Hstep".
+      iApply updN_mono_I.
+      iIntros "[Hmodels Hle2]"; iFrame.
+      iApply interp_local_tys_update; first by done.
+      rewrite -/Σthis -/Σthis1.
+      assert (hno : no_this (subst_ty σt_o omdef.(methodrettype))).
+      { case: hnothis => _.
+        by apply.
+      }
+      rewrite /subst_fty subst_this_no_this_id; last done.
+      rewrite interp_type_subst; last first.
+      { apply bounded_subst with (length odef.(generics)) => //.
+        + apply wf_methods_bounded in hodef.
+          apply hodef in homdef.
+          by apply homdef.
+        + apply inherits_using_wf in hin_t_o => //.
+          destruct hin_t_o as (?& ? & hF & hL); simplify_eq.
+          by rewrite -heq3.
+      }
+      rewrite (interp_type_no_this _ _ _ Σthis Σthis1); last done.
+      assert (hmono:
+        mono (generics tdef) (subst_ty σt_o (methodrettype omdef))).
+      { apply mono_subst with odef.(generics) => //.
+        + apply wf_methods_mono in hodef.
+          apply hodef in homdef.
+          rewrite /wf_mdef_mono hpub in homdef.
+          by apply homdef.
+        + apply wf_methods_bounded in hodef.
+          apply hodef in homdef.
+          by apply homdef.
+        + move => i vi ti hvi hti hc.
+          apply inherits_using_mono with (def := tdef) in hin_t_o => //.
+          elim/mono_classI : hin_t_o => ????; simplify_eq.
+          destruct vi; by eauto.
+        + move => i vi ti hvi hti hc.
+          apply inherits_using_mono with (def := tdef) in hin_t_o => //.
+          elim/mono_classI : hin_t_o => ????; simplify_eq.
+          destruct vi; by eauto.
+      }
+      iApply (interp_with_mono with "hf") => //.
+      { apply wf_ty_subst => //.
+        apply wf_methods_wf in hodef.
         apply hodef in homdef.
-        rewrite /wf_mdef_mono hpub in homdef.
         by apply homdef.
-      + apply wf_methods_bounded in hodef.
-        apply hodef in homdef.
-        by apply homdef.
-      + move => i vi ti hvi hti hc.
-        apply inherits_using_mono with (def := def) in hin_t_o => //.
-        elim/mono_classI : hin_t_o => ????; simplify_eq.
-        destruct vi; by eauto.
-      + move => i vi ti hvi hti hc.
-        apply inherits_using_mono with (def := def) in hin_t_o => //.
-        elim/mono_classI : hin_t_o => ????; simplify_eq.
-        destruct vi; by eauto.
-    }
-    rewrite interp_type_subst; last first.
-    { apply bounded_subst with (length odef.(generics)) => //.
-      + apply wf_methods_bounded in hodef.
-        apply hodef in homdef.
-        by apply homdef.
-      + apply inherits_using_wf in hin_t_o => //.
-        destruct hin_t_o as (?& ? & hF & hL); simplify_eq.
-        by rewrite -heq3.
-    }
-    iApply (interp_with_mono with "hf") => //.
-    { apply wf_ty_subst => //.
-      apply wf_methods_wf in hodef.
-      apply hodef in homdef.
-      by apply homdef.
-    }
-    rewrite -interp_type_subst; last first.
-    { apply bounded_subst with (length odef.(generics)) => //.
-      + apply wf_methods_bounded in hodef.
-        apply hodef in homdef.
-        by apply homdef.
-      + apply inherits_using_wf in hin_t_o => //.
-        destruct hin_t_o as (?&?&hF&?); simplify_eq.
-        by rewrite -heq2.
-    }
-    assert (
-    hmret0 : def1.(constraints) ⊢ methodrettype (subst_mdef σt1_o0 omdef0) <D:
-    methodrettype (subst_mdef σin (subst_mdef σt_o omdef))).
-    { apply subtype_constraint_elim with (Δ' := subst_constraints σt1_o0 odef0.(constraints)) => //.
-      apply subtype_weaken with (Δ := subst_constraints σt1_o0 odef0.(constraints)) => //.
-      by set_solver.
-    }
-    iApply (subtype_is_inclusion _ hΔ1 wf_parent wf_mono wf_constraints_wf wf_constraints_bounded _ _ _ _ hmret0) => //.
-    { apply wf_ty_subst => //.
-      apply wf_methods_wf in hodef0.
-      apply hodef0 in homdef0.
-      by apply homdef0.
-    }
-    rewrite interp_type_subst; last first.
-    { apply wf_methods_bounded in hodef0.
-      apply hodef0 in homdef0.
-      rewrite -heq0.
-      by apply homdef0.
-    }
-    by iApply (expr_soundness _ _ _ _ _ Γ').
+      }
+      rewrite (interp_type_equivI _ _ _ heq_1).
+      rewrite -interp_type_subst; last first.
+      { apply bounded_subst with (length odef.(generics)) => //.
+        + apply wf_methods_bounded in hodef.
+          apply hodef in homdef.
+          by apply homdef.
+        + apply inherits_using_wf in hin_t_o => //.
+          destruct hin_t_o as (?&?&hF&?); simplify_eq.
+          by rewrite -heq2.
+      }
+      assert (hmret0 :
+        def1.(constraints) ⊢ methodrettype (subst_mdef σt1_o0 omdef0) <D:
+        methodrettype (subst_mdef σin (subst_mdef σt_o omdef))).
+      { apply subtype_constraint_elim with (Δ' := subst_constraints σt1_o0 odef0.(constraints)) => //.
+        apply subtype_weaken with (Δ := subst_constraints σt1_o0 odef0.(constraints)) => //.
+        by set_solver.
+      }
+      iApply (subtype_is_inclusion _ hΔ1 wf_parent wf_mono wf_constraints_wf
+        wf_constraints_no_this wf_constraints_bounded wf_fields_wf
+        _ _ _ _ _ hmret0) => //.
+      { apply wf_ty_subst => //.
+        apply wf_methods_wf in hodef0.
+        apply hodef0 in homdef0.
+        by apply homdef0.
+      }
+      rewrite interp_type_subst; last first.
+      { apply wf_methods_bounded in hodef0.
+        apply hodef0 in homdef0.
+        rewrite -heq0.
+        by apply homdef0.
+      }
+      iDestruct (expr_soundness ΔC _ _ _ _ _ Γ' _ omdef0.(methodrettype) ret
+        wf_parent wf_mono wf_constraints_wf wf_constraints_no_this
+        wf_constraints_bounded wf_fields_wf hΔ0 hwfΓ' heval_ret hret
+        with "hmixed1 hmixed0 hΣtΔ0 Hle2") as "hr".
+      assert (heq__:
+        interp_list interp_nothing Σt σt1_o0 ≡ interp_list Σthis1 Σt σt1_o0).
+      { by apply interp_list_no_this. }
+      by rewrite (interp_type_equivI _ _ _ heq__).
   Qed.
 End proofs.
