theories/soundness/priv_call.v
@@ -15,10 +15,8 @@ From shack Require Import eval heap modality interp typing.
 From shack.soundness Require Import expr defs.
 
 Section proofs.
-  (* assume a given set of class definitions *)
-  Context `{PDC: ProgDefContext}.
-  (* assume some SDT constraints and their properties *)
-  Context `{SDTCS: SDTClassSpec}.
+  (* assume a given set of class definitions and their SDT annotations. *)
+  Context `{SDTCVS: SDTClassVarianceSpec}.
 
   (* Helping the inference with this notation that hides pdefs *)
   Local Notation "Δ ⊢ s <: t" := (@subtype _ _ Δ Plain s t) (at level 70, s at next level, no associativity).
@@ -30,92 +28,112 @@ Section proofs.
   (* TODO: keep in sync with call_soundness. Ideally, factor as much as
    * possible and refactor.
    *)
-  Lemma priv_call_soundness C Δ kd rigid Γ lhs t σ name mdef args:
+  Lemma priv_call_soundness C cdef Δ kd rigid Γ lhs name mdef args:
     wf_cdefs pdefs →
     wf_lty Γ →
     Forall wf_constraint Δ →
     Forall (bounded_constraint rigid) Δ →
-    ok_ty Δ (this_type Γ) →
-    type_of_this Γ = (t, σ) →
-    has_method name t C mdef →
+    pdefs !! C = Some cdef →
+    cdef.(classmethods) !! name = Some mdef →
     mdef.(methodvisibility) = Private →
     dom (methodargs mdef) = dom args →
     (∀ (x : string) (ty : lang_ty) (arg : expr),
        methodargs mdef !! x = Some ty →
        args !! x = Some arg →
-       expr_has_ty Δ Γ rigid kd arg (subst_ty σ ty)) →
+       expr_has_ty Δ Γ rigid kd arg ty) →
+    ∀ t tdef Σt σ,
+    pdefs !! t = Some tdef →
+    length Σt = length tdef.(generics) →
+    inherits_using t C σ →
     ∀ Σ st st' n,
     length Σ = rigid →
     cmd_eval C st (CallC lhs ThisE name args) st' n →
+    let Σthis := interp_exact_tag interp_type t Σt in
+    ⌜interp_list interp_nothing Σt σ ≡ Σ⌝ -∗
+    □ interp_env_as_mixed Σt -∗
     □ interp_env_as_mixed Σ -∗
-    □ Σinterp Σ Δ -∗
-    □ (▷ (∀ (a : tag) (a0 : list constraint) (a1 : subtype_kind)
-            (a2 : nat) (a3 : local_tys) (a4 : cmd)
-            (a5 : local_tys),
-            ⌜wf_lty a3⌝ -∗
-            ⌜bounded_lty a2 a3⌝ -∗
-            ⌜ok_ty a0 (this_type a3)⌝ -∗
-            ⌜Forall wf_constraint a0⌝ -∗
-            ⌜Forall (bounded_constraint a2) a0⌝ -∗
-            ∀ (_ : cmd_has_ty a a0 a1 a2 a3 a4 a5)
-              (x0 : list (interp Θ)) (x1 x2 : local_env * heap)
-              (x3 : nat) (_ : length x0 = a2) (_ : cmd_eval a x1 a4 x2 x3),
-              □ interp_env_as_mixed x0 -∗
-              □ Σinterp x0 a0 -∗
-              heap_models x1.2 ∗ interp_local_tys x0 a3 x1.1 -∗
-              |=▷^x3 heap_models x2.2 ∗ interp_local_tys x0 a5 x2.1)) -∗
-    heap_models st.2 ∗ interp_local_tys Σ Γ st.1 -∗
+    □ Σinterp Σthis Σ Δ -∗
+
+    □ ▷ (∀ C Δ kd rigid Γ cmd Γ',
+         ⌜wf_lty Γ⌝ →
+         ⌜bounded_lty rigid Γ⌝ →
+         ⌜Forall wf_constraint Δ⌝ →
+         ⌜Forall (bounded_constraint rigid) Δ⌝ →
+         ∀ t tdef Σt σ,
+         ⌜pdefs !! t = Some tdef⌝ →
+         ⌜length Σt = length tdef.(generics)⌝ →
+         ⌜inherits_using t C σ⌝ →
+         ⌜cmd_has_ty C Δ kd rigid Γ cmd Γ'⌝ →
+         ∀ Σ st st' n,
+         ⌜length Σ = rigid⌝ →
+         ⌜cmd_eval C st cmd st' n⌝ →
+         ⌜interp_list interp_nothing Σt σ ≡ Σ⌝ -∗
+         □ interp_env_as_mixed Σt -∗
+         □ interp_env_as_mixed Σ -∗
+         □ Σinterp (interp_exact_tag interp_type t Σt) Σ Δ -∗
+         heap_models st.2 ∗
+         interp_local_tys (interp_exact_tag interp_type t Σt) Σ Γ st.1 -∗
+         |=▷^n heap_models st'.2 ∗
+               interp_local_tys (interp_exact_tag interp_type t Σt) Σ Γ' st'.1) -∗
+
+    heap_models st.2 ∗ interp_local_tys Σthis Σ Γ st.1 -∗
     |=▷^n heap_models st'.2 ∗
-          interp_local_tys Σ (<[lhs:=subst_ty σ (methodrettype mdef)]> Γ) st'.1.
+          interp_local_tys Σthis Σ (<[lhs:= mdef.(methodrettype)]> Γ) st'.1.
   Proof.
-    move => wfpdefs wflty hΔ hΔb hokthis ht hhasm hpriv hdom hi Σ st st' n hrigid hc.
-    iIntros "#hΣ #hΣΔ #IH".
-    elim/cmd_eval_callI : hc => {n}.
-    move => Ω h h' l t0 vs vargs orig mdef0 run_env run_env' ret n.
-    move => heval_recv hmap hheap hhasm0 hmdom <- heval_body heval_ret.
-    simpl.
+    move => wfpdefs.
     assert (wfpdefs0 := wfpdefs).
     destruct wfpdefs0.
+    move => wflty hΔ hΔb hcdef hmdef hpriv hdom hty_args.
+    move => t tdef Σt σ htdef hlenΣt hin_t_C_σ.
+    move => Σ st st' n hrigid hc /=.
+    iIntros "%heq #hΣt #hΣ #hΣΔ #IH".
+    elim/cmd_eval_callI : hc => {n}.
+    move => Ω h h' l t0 vs vargs orig mdef0 run_env run_env' ret n.
+    move => heval_recv hmap hheap hhasm0 hvis hmdom <- heval_body heval_ret.
+    simpl.
     iIntros "[Hh #Hle]".
-    assert (ht0: this_type Γ = ClassT false t σ).
-    { destruct Γ as [[] Γ].
-      rewrite /this_type /type_of_this /= in ht.
-      rewrite /this_type /type_of_this /=.
-      by injection ht; intros; subst; clear ht.
+    iAssert (□ interp_local_tys (interp_exact_tag interp_type t Σt) Σ Γ Ω)%I as "#Hle_"; first by done.
+    destruct Ω as [vthis Ω].
+    case: heval_recv => hvthis; subst.
+    pose (Σthis := interp_exact_tag interp_type t Σt).
+    iAssert (□ interp_as_mixed interp_nothing)%I as "#hnothing".
+    { iModIntro; by iIntros (w) "hw". }
+    iAssert (□ interp_as_mixed Σthis)%I as "#hΣthis".
+    { rewrite /Σthis.
+      iModIntro; iIntros (w) "hw".
+      iLeft; iRight; iRight.
+      iExists t, Σt, tdef; iSplit; first done.
+      by iApply (exact_subtype_is_inclusion_aux with "hΣt hw").
     }
-    assert (hwfthis_ : wf_ty (ClassT false t σ)).
-    { rewrite -ht0.
-      by apply wflty.
+    iDestruct "Hle_" as "[#Hthis #Hle_]" => /=.
+    iAssert (interp_exact_tag interp_type t Σt (LocV l)) as "#Hl"; first by done.
+    rewrite {3}interp_exact_tag_unseal /interp_exact_tag_def /=.
+    iDestruct "Hthis" as (l0 ? fields ifields H) "(#hconstr & #hf0 & #H◯)".
+    destruct H as ([= <-] & ? & hfields & hidom); simplify_eq.
+    assert (hh: Forall wf_ty σ ∧ length σ = length cdef.(generics) ∧
+      Forall (λ ty : lang_ty, no_this ty) σ).
+    { apply inherits_using_wf in hin_t_C_σ => //.
+      destruct hin_t_C_σ as (? & ?& ? & hh & ?).
+      apply wf_tyI in hh as (? & ? & hlenC & ?); simplify_eq.
+      by eauto.
     }
-    assert (hwfthis: wf_ty (ClassT true t σ)).
-    { by eapply wf_ty_exact. }
-    assert (hwfσ : Forall wf_ty σ) by by apply wf_ty_classI in hwfthis.
-    assert (hcdef : ∃ cdef, pdefs !! C = Some cdef).
-    { apply has_method_from_def in hhasm => //.
-      destruct hhasm as (cdef & _ & hcdef & _).
-      by exists cdef.
+    destruct hh as (hwfσ & hlen & hnothis).
+    assert (hmdefb : mdef_bounded (length cdef.(generics)) mdef).
+    { apply wf_methods_bounded in hcdef.
+      by apply hcdef in hmdef.
     }
-    destruct hcdef as [cdef hcdef].
-    assert (hrecv: expr_has_ty Δ Γ (length Σ) kd ThisE (ClassT false t σ)).
-    { rewrite -ht0.
-      by apply ThisTy.
-    }
-    (* Get inherits relation between dynamic tag and static tag *)
-    iDestruct (expr_soundness Δ (length Σ) Σ _ ThisE with "hΣ hΣΔ Hle") as "#Hrecv" => //.
-    rewrite interp_class_unfold //.
-    iDestruct "Hrecv" as (? t1 def def1 σin Σt fields ifields) "(%Hpure & _ & _ & _ & _ & Hl)".
-    destruct Hpure as ([= <-] & hdef & hdef1 & ? & hin_t1_t & hfields & hidom).
     iDestruct "Hh" as (sh) "(H● & %Hdom & #Hh)".
-    iDestruct (sem_heap_own_valid_2 with "H● Hl") as "#HΦ".
+    iDestruct (sem_heap_own_valid_2 with "H● H◯") as "#HΦ".
     iDestruct ("Hh" with "[//]") as (?) "[H H▷]".
     iRewrite "H" in "HΦ".
     rewrite option_equivI prod_equivI /=.
     iDestruct "HΦ" as "[%Ht HΦ]".
     fold_leibniz; subst.
+    assert (hhasm : has_method name C C mdef) by by econstructor.
     destruct (has_method_ordered _ _ _ _ _ _ _ _ wf_override wf_parent
-      wf_constraints_bounded wf_methods_bounded hin_t1_t hhasm0 hhasm)
+      wf_constraints_bounded wf_methods_bounded hin_t_C_σ hhasm0 hhasm)
     as (odef0 & odef & σt1_o0 & σt_o & omdef0 & omdef & hodef0 & hodef & homdef0 & homdef & hin_t1_o0
-    & hin_t_o & -> & -> & (*hpub0 &*) hincl0 & [hh | hh]); last first.
+        & hin_t_o & -> & -> & (*hpub0 &*) hincl0 & [hh | hh]); last first.
     (* TODO: update this when proper private methods are implemented *)
     { destruct hh as (σ_ & hin_ & _).
       assert (hin__: inherits_using orig C (subst_ty σ_ <$> σt_o)).
@@ -124,211 +142,149 @@ Section proofs.
       rewrite hpriv.
       by intro hf; elim hf.
     }
-    destruct hh as (_ & -> & -> & <-); simplify_eq.
+    destruct hh as (_ & -> & -> & <-).
+    assert (h0 : subst_mdef σt_o omdef = omdef).
+    { apply inherits_using_refl in hin_t_o => //.
+      destruct hin_t_o as (? & ? & ->); simplify_eq.
+      apply subst_mdef_gen_targs.
+      by rewrite H.
+    }
+    rewrite !h0 in hty_args, hdom, hpriv, hmdef hmdefb.
+    assert (h1: mdef_bounded (length σt_o) omdef).
+    { apply inherits_using_wf in hin_t_o => //.
+      destruct hin_t_o as (? & ? & ? & hwf & ?); simplify_eq.
+      apply wf_tyI in hwf as (? & ? & hlen0 & ?); simplify_eq.
+      by rewrite hlen0.
+    }
+    rewrite -subst_mdef_mdef in hhasm0; last done.
+    rewrite -!subst_mdef_mdef in heval_ret => //.
+    rewrite h0 in heval_ret.
+    rewrite -subst_mdef_mdef in heval_body; last done.
+    rewrite h0 in heval_body.
+    rewrite -subst_mdef_mdef in hvis; last done.
+    rewrite h0 in hvis.
+    rewrite -subst_mdef_mdef in hmdom; last done.
+    rewrite h0 in hmdom.
+    rewrite h0.
+    clear hin_t1_o0 hin_t_o hincl0 hhasm hhasm0 h0 h1 σt_o.
+    simplify_eq.
     (* END TODO *)
-    assert (hh: Forall wf_ty σt_o ∧ length cdef.(generics) = length σt_o).
-    { apply inherits_using_wf in hin_t_o => //.
-      destruct hin_t_o as (?&?&?&hh).
-      split; first by apply wf_ty_classI in hh.
-      apply wf_tyI in hh as (? & ? & ? & ?); by simplify_eq.
-    }
-    destruct hh as [hFσt_o heq1].
-    assert (hokc: ok_ty cdef.(constraints) (ClassT false C (gen_targs (length cdef.(generics))))).
-    { econstructor => //.
-      - move => k ty hty.
-        apply lookup_gen_targs in hty as ->.
-        by constructor.
-      - move => k [c0 c1] hc /=.
-        rewrite !subst_ty_id.
-        + apply SubConstraint.
-          by apply elem_of_list_lookup_2 in hc.
-        + apply wf_constraints_bounded in hcdef.
-          rewrite /wf_cdef_constraints_bounded Forall_lookup in hcdef.
-          by apply hcdef in hc as [].
-        + apply wf_constraints_bounded in hcdef.
-          rewrite /wf_cdef_constraints_bounded Forall_lookup in hcdef.
-          by apply hcdef in hc as [].
-    }
-    assert (hF: Forall (bounded (length σ)) σt_o).
-    { apply inherits_using_wf in hin_t_o => //.
-      destruct hin_t_o as (? & ? & ? & ?); simplify_eq.
-      apply wf_tyI in hwfthis as (? & ? & hlen & ?); simplify_eq.
-      by rewrite hlen.
-    }
-    assert (hh: wf_mdef_ty C cdef.(constraints) (length cdef.(generics)) (gen_targs (length cdef.(generics))) omdef).
+    pose (CT := ClassT false C (gen_targs (length cdef.(generics)))).
+    pose (ΔC := (ThisT, CT) :: cdef.(constraints)).
+    assert (hh: wf_mdef_ty C ΔC (length cdef.(generics)) omdef).
     { apply wf_mdefs in hcdef.
       by apply hcdef in homdef0.
     }
     destruct hh as (Γ' & hwfΓ' & hbody & hret).
-    assert (hwf_lty0 : wf_lty
-    {|
-      type_of_this := (C, gen_targs (length cdef.(generics)));
-      ctxt := methodargs omdef
-    |}).
-    { split.
-      - rewrite /this_type /=.
-        econstructor => //; first by rewrite length_gen_targs.
-        by apply gen_targs_wf_2.
-      - rewrite map_Forall_lookup => k tk hk.
-        apply wf_methods_wf in hcdef.
-        apply hcdef in homdef0.
-        by apply homdef0 in hk.
+    assert (hwf_lty0 : wf_lty omdef.(methodargs)).
+    { apply wf_methods_wf in hcdef.
+      apply hcdef in homdef0.
+      by apply homdef0.
     }
-    assert (hbounded : bounded_lty (length cdef.(generics))
-    {|
-      type_of_this := (C, gen_targs (length cdef.(generics)));
-      ctxt := methodargs omdef
-    |}).
-    { split => /=.
-      - rewrite /this_type /=.
-        constructor.
-        by apply bounded_gen_targs.
-      - rewrite map_Forall_lookup => k tk hk.
-        apply wf_methods_bounded in hcdef.
-        apply hcdef in homdef0.
-        by apply homdef0 in hk.
+    assert (hbounded : bounded_lty (length cdef.(generics)) omdef.(methodargs)).
+    { apply wf_methods_bounded in hcdef.
+      apply hcdef in homdef0.
+      by apply homdef0.
     }
-    assert (hΔ1 : Forall wf_constraint def1.(constraints)).
-    { by apply wf_constraints_wf in hdef1.  }
+    assert (hΔt : Forall wf_constraint tdef.(constraints)).
+    { by apply wf_constraints_wf in htdef.  }
     apply cmd_eval_subst in heval_body.
     rewrite expr_eval_subst in heval_ret.
     iModIntro; iNext.
-    iAssert (□ interp_env_as_mixed (interp_list Σ (subst_ty σ <$> σt_o)))%I as "#hΣc".
-    { iModIntro.
-      iIntros (k ϕ hk v) "hv".
-      apply list_lookup_fmap_inv in hk as [ty0 [-> h0]].
-      apply list_lookup_fmap_inv in h0 as [ty1 [-> h1]].
-      iDestruct (submixed_is_inclusion_aux with "hΣ hv") as "hh".
-      - apply wf_ty_subst => //.
-        rewrite Forall_lookup in hFσt_o; by eapply hFσt_o.
+    assert (heq2: interp_list interp_nothing Σt σ ≡ interp_list interp_nothing Σt σ) by done.
+    iAssert (□ interp_env_as_mixed (interp_list interp_nothing Σt σ))%I as "#hΣc".
+    { iModIntro; iIntros (k phi hk w) "hw".
+      apply list_lookup_fmap_inv in hk as [ty [-> hk]].
+      iDestruct (submixed_is_inclusion_aux with "hnothing hΣt hw") as "hh".
+      - rewrite Forall_lookup in hwfσ; by apply hwfσ in hk.
       - by rewrite interp_mixed_unfold.
     }
-    assert (hokt: ok_ty Δ (ClassT true t σ)).
-    { destruct Γ as [[] ?].
-      rewrite /this_type /= in ht, hokthis.
-      injection ht; intros; subst; clear ht.
-      by eapply ok_ty_exact.
+    iAssert (□ Σinterp Σthis Σt tdef.(constraints))%I as "#hΣtc".
+    { iModIntro; iIntros (k0 c0 hc0 w) "h0".
+      assert (hc0' := hc0).
+      apply wf_constraints_no_this in htdef.
+      rewrite /wf_cdef_constraints_no_this Forall_lookup in htdef.
+      apply htdef in hc0' as [].
+      rewrite (interp_type_no_this _ _ _ Σthis interp_nothing); last done.
+      rewrite (interp_type_no_this _ _ _ Σthis interp_nothing); last done.
+      by iApply "hconstr".
     }
-    assert (hok0: ok_ty (Δ ++ subst_constraints σ (constraints def)) (ClassT true C (subst_ty σ <$> σt_o))).
-    { econstructor => //.
-      - move => k ty hk.
-        apply list_lookup_fmap_inv in hk as [ty0 [-> h0]].
-        eapply ok_ty_subst => //.
-        + apply inherits_using_ok in hin_t_o => //.
-          destruct hin_t_o as (tdef & htdef & hokC); simplify_eq.
-          apply ok_tyI in hokC as (? & ? & hokC & ?).
-          by apply hokC in h0.
-        + rewrite Forall_lookup in hFσt_o; by eapply hFσt_o.
-        + apply ok_tyI in hokt as (? & ? & hokt & ?).
-          apply Forall_lookup => ? ty hl.
-          by apply hokt in hl.
-      - move => k [c0 c1] hc /=.
-        assert (h0 := hcdef).
-        apply wf_constraints_bounded in h0.
-        rewrite /wf_cdef_constraints_bounded Forall_lookup in h0.
-        rewrite -!subst_ty_subst.
-        + apply subtype_weaken with (Δ := subst_constraints σ def.(constraints)); last by set_solver.
-          apply subtype_subst => //.
-          apply inherits_using_ok in hin_t_o => //.
-          destruct hin_t_o as (tdef & htdef & hokC); simplify_eq.
-          apply ok_tyI in hokC as (? & ? & ? & hokC); simplify_eq.
-          by apply hokC in hc.
-        + rewrite -heq1; by apply h0 in hc as [].
-        + rewrite -heq1; by apply h0 in hc as [].
-    }
-    assert (hok0_: ok_ty Δ (ClassT true C (subst_ty σ <$> σt_o))).
-    { eapply ok_ty_constraint_trans with (kd := Aware); first by apply hok0.
-      move => k c hc /=.
-      rewrite lookup_app in hc.
-      destruct (Δ !! k) as [c0 | ] eqn:hc0.
-      - case : hc => <-.
-        apply SubConstraint.
-        apply elem_of_list_lookup_2 in hc0.
-        by destruct c0.
-      - apply list_lookup_fmap_inv in hc as [c1 [-> hc1]].
-        rewrite /subst_constraint /=.
-        apply ok_tyI in hokt as (? & ? & ? & hokt); simplify_eq.
-        by apply hokt in hc1.
-    }
-    iAssert (□ Σinterp (interp_list Σ (subst_ty σ <$> σt_o)) (constraints cdef))%I as "#hΣΔc".
+    iAssert (□ Σinterp (interp_exact_tag interp_type t Σt)
+               (interp_list interp_nothing Σt σ)
+               ΔC)%I as "#hΣΔc".
     { iModIntro.
       iIntros (k c hc v) "hv".
-      apply ok_tyI in hok0_ as (? & ? & ? & hok); simplify_eq.
+      destruct k as [ | k]; simpl in hc.
+      { assert (heq_:
+          interp_list (interp_exact_tag interp_type t Σt)
+            (interp_list interp_nothing Σt σ) (gen_targs (length (generics cdef))) ≡
+            (interp_list interp_nothing Σt σ)).
+        { apply interp_list_gen_targs.
+          by rewrite /interp_list fmap_length.
+        }
+        case : hc => <- /=.
+        rewrite /ΔC /CT interp_this_unfold interp_tag_unfold.
+        rewrite (interp_tag_equivI _ _ heq_ C v).
+        iDestruct ((exact_subtype_is_inclusion_aux _ _ _ _ htdef hlenΣt) with "hΣt hv") as "hv".
+        by iApply tag_inherits_using_is_inclusion.
+      }
+      apply inherits_using_ok in hin_t_C_σ => //.
+      destruct hin_t_C_σ as (? & ? & hokC); simplify_eq.
+      apply ok_tyI in hokC as(? & ? & ? & hok); simplify_eq.
       assert (hc' := hc).
       apply hok in hc'.
-      iDestruct ((subtype_is_inclusion _ hΔ wf_parent wf_mono wf_constraints_wf
-        wf_constraints_bounded _ _ _ _ hc') with "hΣ hΣΔ") as "hh"; try assumption.
-      { apply wf_ty_subst; first by apply wf_ty_subst_map.
+      iDestruct ((subtype_is_inclusion _ hΔt wf_parent wf_mono wf_constraints_wf
+        wf_constraints_no_this wf_constraints_bounded wf_fields_wf _ _ _ _ _ hc' v) with "hΣthis hΣt hΣtc") as "hh".
+      { apply wf_ty_subst; first done.
         apply wf_constraints_wf in hcdef.
         rewrite /wf_cdef_constraints_wf Forall_lookup in hcdef.
         by apply hcdef in hc as [].
       }
-      assert (hbc: bounded_constraint (length (subst_ty σ <$> σt_o)) c).
+      assert (hbc: bounded_constraint (length σ) c).
       { apply wf_constraints_bounded in hcdef.
         rewrite /wf_cdef_constraints_bounded Forall_lookup in hcdef.
-        rewrite map_length -heq1.
+        rewrite hlen.
         by apply hcdef in hc.
       }
       destruct hbc as [].
       rewrite interp_type_subst; last done.
       rewrite interp_type_subst; last done.
+      assert (heq_: interp_list Σthis Σt σ ≡ interp_list interp_nothing Σt σ).
+      { by apply interp_list_no_this. }
+      rewrite (interp_type_equivI _ _ _ heq_).
+      rewrite (interp_type_equivI _ _ _ heq_).
       by iApply "hh".
     }
-    assert (hlc:
-      length (interp_list Σ (subst_ty σ <$> σt_o)) = length cdef.(generics)).
-    { by rewrite /interp_list !fmap_length heq1. }
-    assert (hentails_cdef: ∀ k s t,
-      cdef.(constraints) !! k = Some (s, t) → cdef.(constraints) ⊢ s <: t).
-    { move => ??? hc.
-      eapply SubConstraint.
-      by apply elem_of_list_lookup_2 in hc.
+    assert (hlc: length (interp_list interp_nothing Σt σ) = length cdef.(generics)).
+    { by rewrite /interp_list !fmap_length. }
+    assert (hwfΔc: Forall wf_constraint ((ThisT, CT) :: cdef.(constraints))).
+    { apply Forall_cons; split.
+      - split => //=.
+        econstructor => //; first by rewrite length_gen_targs.
+        by apply gen_targs_wf_2.
+      - by apply wf_constraints_wf in hcdef.
     }
-    assert (hwfΔc: Forall wf_constraint cdef.(constraints)).
-    { by apply wf_constraints_wf in hcdef. }
-    assert (hbΔc: Forall (bounded_constraint (length cdef.(generics))) cdef.(constraints)).
-    { by apply wf_constraints_bounded in hcdef. }
-    iSpecialize ("IH" $! C _ Plain (length cdef.(generics)) _ _ _ hwf_lty0 hbounded hokc hwfΔc hbΔc
-    hbody (interp_list Σ (subst_ty σ <$> σt_o))  _ _ _ hlc heval_body with "hΣc hΣΔc"); simpl.
-    iDestruct ("IH" with "[Hh Hle H●]") as "Hstep".
+    assert (hbΔc: Forall (bounded_constraint (length cdef.(generics))) ((ThisT, CT) :: cdef.(constraints))).
+    { apply Forall_cons; split.
+      - split => //=.
+        constructor.
+        by apply bounded_gen_targs.
+      - by apply wf_constraints_bounded in hcdef.
+    }
+    iSpecialize ("IH" $! C _ Plain (length cdef.(generics)) _ _ _ hwf_lty0 hbounded hwfΔc hbΔc).
+    iSpecialize ("IH" $! t tdef Σt σ htdef hlenΣt hin_t_C_σ hbody (interp_list interp_nothing Σt σ)).
+    iSpecialize ("IH" $! _ _ _ hlc heval_body heq2 with "hΣt hΣc hΣΔc"); simpl.
+    iDestruct ("IH" with "[Hh Hle_ H●]") as "Hstep".
     { iClear "IH"; iSplit.
       - iExists _; iFrame.
         iSplit; last done.
         by rewrite Hdom.
-      - iSplit => /=.
-        + iDestruct ((this_inherits_using_is_inclusion wf_parent Σ _ _ σ _ (LocV l) hin_t_o)) as "hh" => //.
-          destruct Γ as [[? ?] Γ].
-          destruct Ω as [vthis Ω].
-          rewrite /type_of_this in ht.
-          injection ht; intros; subst; clear ht.
-          iDestruct "Hle" as "[hthis _]".
-          simpl in heval_recv.
-          case: heval_recv => ->.
-          simpl.
-          iDestruct ("hh" with "hthis") as "hh2".
-          iClear "hΣ hΣΔ hthis Hl Hh HΦ H H▷ hh H●".
-          rewrite /interp_this_type.
-          rewrite interp_this_equivI; first done.
-          rewrite list_equiv_lookup => k.
-          rewrite !list_lookup_fmap.
-          destruct (decide (k < length cdef.(generics))) as [hlt | hge].
-          * assert (hh: is_Some (σt_o !! k)).
-            { rewrite heq1 in hlt.
-              by apply lookup_lt_is_Some_2 in hlt.
-            }
-            destruct hh as [ty hty]; rewrite hty /=.
-            rewrite lookup_seq_lt //=.
-            f_equiv => w.
-            by rewrite interp_generic_unfold /interp_generic /=
-              !list_lookup_fmap hty.
-          * assert (hle: length cdef.(generics) ≤ k) by lia.
-            rewrite lookup_seq_ge //=.
-            rewrite heq1 in hle.
-            by apply lookup_ge_None_2 in hle as ->.
+      - iSplit => /=; first done.
         + iIntros (v ty hv).
           assert (ha: ∃ arg, args !! v = Some arg).
           { apply elem_of_dom.
             rewrite /subst_mdef /= !dom_fmap_L in hmdom.
-            rewrite -hdom /subst_mdef /= dom_fmap.
+            rewrite -hdom.
             by apply elem_of_dom.
           }
           destruct ha as [arg ha].
@@ -342,43 +298,16 @@ Section proofs.
           destruct hvarg as [varg hvarg].
           iExists varg; rewrite hvarg; iSplitR; first done.
           rewrite (map_args_lookup _ _ _ args vargs hmap v) ha /= in hvarg.
-          destruct (methodargs omdef !! v) as [tw | ] eqn:htw => //.
-          case: hv => <-; clear ty.
-          assert (h0: methodargs (subst_mdef σt_o omdef) !! v = Some (subst_ty σt_o tw)).
-          { by rewrite /subst_mdef /= !lookup_fmap htw. }
-          move: (hi v _ _ h0 ha) => haty.
-          iDestruct (expr_soundness with "hΣ hΣΔ Hle") as "he" => //.
-          assert (hb: bounded (length σt_o) tw).
-          { apply wf_methods_bounded in hcdef.
-            apply hcdef in homdef0.
-            apply homdef0 in htw.
-            by rewrite -heq1.
-          }
-          rewrite interp_type_subst; last by eapply bounded_subst.
-          rewrite interp_type_subst; last done.
-          rewrite interp_type_equivI; first done.
-          rewrite /interp_list -list_fmap_compose.
-          apply list_fmap_equiv_ext => k ty hty w /=.
-          rewrite interp_type_subst; first done.
-          apply inherits_using_wf in hin_t_o => //.
-          destruct hin_t_o as (? & ? & hB & ?); simplify_eq.
-          rewrite Forall_lookup in hB.
-          apply hB in hty.
-          apply wf_tyI in hwfthis as (? & ? & hlen & ?); simplify_eq.
-          by rewrite hlen.
+          move: (hty_args v _ _ hv ha) => haty.
+          iDestruct (expr_soundness with "hΣthis hΣ hΣΔ Hle") as "he" => //.
+          by rewrite (interp_type_equivI _ _ _ heq).
     }
     iRevert "Hstep".
     iApply updN_mono_I.
     iIntros "[Hmodels Hle2]"; iFrame.
     iApply interp_local_tys_update; first by done.
-    assert (hb : bounded (length σt_o) (methodrettype omdef)).
-    { apply wf_methods_bounded in hcdef.
-      apply hcdef in homdef0.
-      rewrite -heq1.
-      by apply homdef0.
-    }
-    rewrite subst_ty_subst; last done.
-    rewrite interp_type_subst; last by rewrite map_length.
-    by iApply (expr_soundness _ _ (interp_list Σ (subst_ty σ <$> σt_o)) _ _ Γ').
+    iDestruct ((expr_soundness ΔC _ Σthis (interp_list interp_nothing Σt σ)  _ _ Γ' run_env') with "hΣthis hΣc hΣΔc") as "hr" => //.
+    rewrite (interp_type_equivI _ _ _ heq).
+    by iApply "hr".
   Qed.
 End proofs.
